spec/capDL/CSpace_D.thy
@@ -478,8 +478,8 @@ definition cdl_default_tcb :: "cdl_object"
 where "cdl_default_tcb \<equiv>  Tcb \<lparr>cdl_tcb_caps =
            [tcb_cspace_slot \<mapsto> cdl_cap.NullCap, tcb_vspace_slot \<mapsto> cdl_cap.NullCap, tcb_replycap_slot \<mapsto>
             cdl_cap.NullCap, tcb_caller_slot \<mapsto> cdl_cap.NullCap, tcb_ipcbuffer_slot \<mapsto> cdl_cap.NullCap,
-            tcb_pending_op_slot \<mapsto> cdl_cap.NullCap, tcb_boundntfn_slot \<mapsto> cdl_cap.NullCap],
-           cdl_tcb_fault_endpoint = 0,
+            tcb_fault_handler_slot \<mapsto> cdl_cap.NullCap, tcb_pending_op_slot \<mapsto> cdl_cap.NullCap,
+            tcb_boundntfn_slot \<mapsto> cdl_cap.NullCap],
            cdl_tcb_intent =
              \<lparr>cdl_intent_op = None, cdl_intent_error = False,cdl_intent_cap = 0, cdl_intent_extras = [],
                 cdl_intent_recv_slot = None\<rparr>, cdl_tcb_has_fault = False, cdl_tcb_domain = minBound\<rparr>"
